Change device.run1 to use TL interface (#942)

cava2/TLUL.v
@@ -101,18 +101,16 @@ Section Var.
   (*   PutPartialData = 3'h 1, *)
   (*   Get            = 3'h 4 *)
   (* } tl_a_op_e; *)
-  Definition tl_a_op_e      := BitVec 3.
-  Definition PutFullData    := Constant tl_a_op_e 0.
-  Definition PutPartialData := Constant tl_a_op_e 1.
-  Definition Get            := Constant tl_a_op_e 4.
+  Definition PutFullData    := 0.
+  Definition PutPartialData := 1.
+  Definition Get            := 4.
 
   (* typedef enum logic [2:0] { *)
   (*   AccessAck     = 3'h 0, *)
   (*   AccessAckData = 3'h 1 *)
   (* } tl_d_op_e; *)
-  Definition tl_d_op_e     := BitVec 3.
-  Definition AccessAck     := Constant tl_d_op_e 0.
-  Definition AccessAckData := Constant tl_d_op_e 1.
+  Definition AccessAck     := 0.
+  Definition AccessAckData := 1.
 
   Definition io_req : type :=
     Bit **          (* read *)
@@ -152,9 +150,9 @@ Section Var.
       let a_ack := a_valid && !outstanding in
       let d_ack := outstanding && d_ready in
 
-      let rd_req := a_ack && a_opcode == `Get` in
+      let rd_req := a_ack && a_opcode == `K Get` in
       let wr_req := a_ack &&
-        (a_opcode == `PutFullData` || a_opcode == `PutPartialData`) in
+        (a_opcode == `K PutFullData` || a_opcode == `K PutPartialData`) in
 
       (* TODO(blaxill): skipping malformed tl packet detection *)
       let err_internal := `Zero` in
@@ -164,7 +162,7 @@ Section Var.
         if a_ack then
           ( a_source
           , a_size
-          , if rd_req then `AccessAckData` else `AccessAck`
+          , if rd_req then `K AccessAckData` else `K AccessAck`
           , error_i || err_internal
           , `One`
           )
@@ -200,3 +198,109 @@ Section Var.
   }}.
 
 End Var.
+
+Definition tl_h2d := denote_type tl_h2d_t.
+Definition tl_h2d_default := default (t := tl_h2d_t).
+
+Ltac destruct_tl_h2d_step :=
+  let t1 := eval unfold tl_h2d in tl_h2d in
+  let t2 := eval simpl in t1 in
+  match goal with
+  | v : tl_h2d |- _ => unfold tl_h2d in v
+  | v : t1 |- _ => simpl in v
+  | v : t2 |- _ =>
+    destruct v as (?a_valid, (?a_opcode, (?a_param, (?a_size, (?a_source,
+                  (?a_address, (?a_mask, (?a_data, (?a_user, ?d_ready)))))))))
+  end.
+Ltac destruct_tl_h2d := repeat destruct_tl_h2d_step.
+
+Definition a_valid   (h2d: tl_h2d) : bool := ltac:(destruct_tl_h2d; apply a_valid).
+Definition a_opcode  (h2d: tl_h2d) : N := ltac:(destruct_tl_h2d; apply a_opcode).
+Definition a_param   (h2d: tl_h2d) : N := ltac:(destruct_tl_h2d; apply a_param).
+Definition a_size    (h2d: tl_h2d) : N := ltac:(destruct_tl_h2d; apply a_size).
+Definition a_source  (h2d: tl_h2d) : N := ltac:(destruct_tl_h2d; apply a_source).
+Definition a_address (h2d: tl_h2d) : N := ltac:(destruct_tl_h2d; apply a_address).
+Definition a_mask    (h2d: tl_h2d) : N := ltac:(destruct_tl_h2d; apply a_mask).
+Definition a_data    (h2d: tl_h2d) : N := ltac:(destruct_tl_h2d; apply a_data).
+Definition a_user    (h2d: tl_h2d) : N := ltac:(destruct_tl_h2d; apply a_user).
+Definition d_ready   (h2d: tl_h2d) : bool := ltac:(destruct_tl_h2d; apply d_ready).
+
+Ltac tl_h2d_setter v h2d x :=
+  unfold tl_h2d in h2d; simpl in h2d;
+  destruct h2d as (a_valid', (a_opcode', (a_param', (a_size', (a_source',
+                  (a_address', (a_mask', (a_data', (a_user', d_ready')))))))));
+  let setter :=
+      (match eval pattern x in (a_valid', (a_opcode', (a_param', (a_size', (a_source',
+                  (a_address', (a_mask', (a_data', (a_user', d_ready'))))))))) with
+       | ?set_x _ => constr:(set_x v)
+       end) in
+  exact setter.
+
+Definition set_a_valid   : bool -> tl_h2d -> tl_h2d := ltac:(intros v h2d; tl_h2d_setter v h2d a_valid').
+Definition set_a_opcode  : N -> tl_h2d -> tl_h2d := ltac:(intros v h2d; tl_h2d_setter v h2d a_opcode').
+Definition set_a_param   : N -> tl_h2d -> tl_h2d := ltac:(intros v h2d; tl_h2d_setter v h2d a_param').
+Definition set_a_size    : N -> tl_h2d -> tl_h2d := ltac:(intros v h2d; tl_h2d_setter v h2d a_size').
+Definition set_a_source  : N -> tl_h2d -> tl_h2d := ltac:(intros v h2d; tl_h2d_setter v h2d a_source').
+Definition set_a_address : N -> tl_h2d -> tl_h2d := ltac:(intros v h2d; tl_h2d_setter v h2d a_address').
+Definition set_a_mask    : N -> tl_h2d -> tl_h2d := ltac:(intros v h2d; tl_h2d_setter v h2d a_mask').
+Definition set_a_data    : N -> tl_h2d -> tl_h2d := ltac:(intros v h2d; tl_h2d_setter v h2d a_data').
+Definition set_a_user    : N -> tl_h2d -> tl_h2d := ltac:(intros v h2d; tl_h2d_setter v h2d a_user').
+Definition set_d_ready   : bool -> tl_h2d -> tl_h2d := ltac:(intros v h2d; tl_h2d_setter v h2d d_ready').
+
+Definition tl_d2h := denote_type tl_d2h_t.
+Definition tl_d2h_default := default (t := tl_d2h_t).
+
+Ltac destruct_tl_d2h_step :=
+  let t1 := eval unfold tl_d2h in tl_d2h in
+  let t2 := eval simpl in t1 in
+  match goal with
+  | v : tl_d2h |- _ => unfold tl_d2h in v
+  | v : t1 |- _ => simpl in v
+  | v : t2 |- _ =>
+    destruct v as (?d_valid, (?d_opcode, (?d_param, (?d_size, (?d_source,
+                  (?d_sink, (?d_data, (?d_user, (?d_error, ?a_ready)))))))))
+  end.
+
+Ltac destruct_tl_d2h := repeat destruct_tl_d2h_step.
+
+Definition d_valid  (d2h : tl_d2h) : bool := ltac:(destruct_tl_d2h; apply d_valid).
+Definition d_opcode (d2h : tl_d2h) : N := ltac:(destruct_tl_d2h; apply d_opcode).
+Definition d_param  (d2h : tl_d2h) : N := ltac:(destruct_tl_d2h; apply d_param).
+Definition d_size   (d2h : tl_d2h) : N := ltac:(destruct_tl_d2h; apply d_size).
+Definition d_source (d2h : tl_d2h) : N := ltac:(destruct_tl_d2h; apply d_source).
+Definition d_sink   (d2h : tl_d2h) : N := ltac:(destruct_tl_d2h; apply d_sink).
+Definition d_data   (d2h : tl_d2h) : N := ltac:(destruct_tl_d2h; apply d_data).
+Definition d_user   (d2h : tl_d2h) : N := ltac:(destruct_tl_d2h; apply d_user).
+Definition d_error  (d2h : tl_d2h) : bool := ltac:(destruct_tl_d2h; apply d_error).
+Definition a_ready  (d2h : tl_d2h) : bool := ltac:(destruct_tl_d2h; apply a_ready).
+
+Ltac tl_d2h_setter v d2h x :=
+  unfold tl_d2h in d2h; simpl in d2h;
+  destruct d2h as (d_valid', (d_opcode', (d_param', (d_size', (d_source',
+                  (d_sink', (d_data', (d_user', (d_error', a_ready')))))))));
+  let setter :=
+      (match eval pattern x in (d_valid', (d_opcode', (d_param', (d_size', (d_source',
+                               (d_sink', (d_data', (d_user', (d_error', a_ready'))))))))) with
+       | ?set_x _ => constr:(set_x v)
+       end) in
+  exact setter.
+
+Definition set_d_valid  : bool -> tl_d2h -> tl_d2h := ltac:(intros v d2h; tl_d2h_setter v d2h d_valid').
+Definition set_d_opcode : N -> tl_d2h -> tl_d2h := ltac:(intros v d2h; tl_d2h_setter v d2h d_opcode').
+Definition set_d_param  : N -> tl_d2h -> tl_d2h := ltac:(intros v d2h; tl_d2h_setter v d2h d_param').
+Definition set_d_size   : N -> tl_d2h -> tl_d2h := ltac:(intros v d2h; tl_d2h_setter v d2h d_size').
+Definition set_d_source : N -> tl_d2h -> tl_d2h := ltac:(intros v d2h; tl_d2h_setter v d2h d_source').
+Definition set_d_sink   : N -> tl_d2h -> tl_d2h := ltac:(intros v d2h; tl_d2h_setter v d2h d_sink').
+Definition set_d_data   : N -> tl_d2h -> tl_d2h := ltac:(intros v d2h; tl_d2h_setter v d2h d_data').
+Definition set_d_user   : N -> tl_d2h -> tl_d2h := ltac:(intros v d2h; tl_d2h_setter v d2h d_user').
+Definition set_d_error  : bool -> tl_d2h -> tl_d2h := ltac:(intros v d2h; tl_d2h_setter v d2h d_error').
+Definition set_a_ready  : bool -> tl_d2h -> tl_d2h := ltac:(intros v d2h; tl_d2h_setter v d2h a_ready').
+
+Ltac tlsimpl :=
+  unfold tl_h2d_default, tl_d2h_default in *; simpl Types.default in *;
+  cbn [set_a_valid set_a_opcode set_a_param set_a_size set_a_source
+       set_a_address set_a_mask set_a_data set_a_user set_d_ready
+       a_valid a_opcode a_param a_size a_source a_address a_mask a_data a_user d_ready
+       set_d_valid set_d_opcode set_d_param set_d_size set_d_source
+       set_d_sink set_d_data set_d_user set_d_error set_a_ready
+       d_valid d_opcode d_param d_size d_source d_sink d_data d_user d_error a_ready] in *.
